src/BoundedArithmetic/Pow2BaseProofs.v
@@ -9,11 +9,12 @@ Require Import Crypto.Util.Tactics.BreakMatch.
 Require Import Crypto.Util.Tactics.UniquePose.
 Require Import Crypto.Util.Tactics.RewriteHyp.
 Require Import Crypto.BoundedArithmetic.Pow2Base.
-Require Import Crypto.BoundedArithmetic.BaseSystemProofs.
 Require Import Crypto.Util.Notations.
 Require Export Crypto.Util.Bool.
 Require Export Crypto.Util.FixCoqMistakes.
 Local Open Scope Z_scope.
+
+Require Crypto.BoundedArithmetic.BaseSystemProofs.
 
 Create HintDb simpl_add_to_nth discriminated.
 Create HintDb push_upper_bound discriminated.
@@ -65,12 +66,6 @@ Section Pow2BaseProofs.
     apply fold_right_invariant; try omega.
     eauto using Z.add_nonneg_nonneg, limb_widths_nonneg, In_firstn.
   Qed. Hint Resolve sum_firstn_limb_widths_nonneg.
-
-  Lemma two_sum_firstn_limb_widths_pos n : 0 < 2^sum_firstn limb_widths n.
-  Proof using Type*. auto with zarith. Qed.
-
-  Lemma two_sum_firstn_limb_widths_nonzero n : 2^sum_firstn limb_widths n <> 0.
-  Proof using Type*. pose proof (two_sum_firstn_limb_widths_pos n); omega. Qed.
 
   Lemma base_from_limb_widths_step : forall i b w, (S i < length limb_widths)%nat ->
     nth_error base i = Some b ->
@@ -133,50 +128,6 @@ Section Pow2BaseProofs.
     reflexivity.
   Qed.
 
-  Lemma base_succ : forall i, ((S i) < length limb_widths)%nat ->
-    nth_default 0 base (S i) mod nth_default 0 base i = 0.
-  Proof using Type*.
-    intros.
-    repeat rewrite nth_default_base by omega.
-    apply Z.mod_same_pow.
-    split; [apply sum_firstn_limb_widths_nonneg | ].
-    destruct (NPeano.Nat.eq_dec i 0); subst.
-      + case_eq limb_widths; intro; unfold sum_firstn; simpl; try omega; intros l' lw_eq.
-        apply Z.add_nonneg_nonneg; try omega.
-        apply limb_widths_nonneg.
-        rewrite lw_eq.
-        apply in_eq.
-      + assert (i < length limb_widths)%nat as i_lt_length by omega.
-        apply nth_error_length_exists_value in i_lt_length.
-        destruct i_lt_length as [x nth_err_x].
-        erewrite sum_firstn_succ; eauto.
-        apply nth_error_value_In in nth_err_x.
-        apply limb_widths_nonneg in nth_err_x.
-        omega.
-   Qed.
-
-   Lemma nth_error_subst : forall i b, nth_error base i = Some b ->
-     b = 2 ^ (sum_firstn limb_widths i).
-   Proof using Type*.
-     intros i b nth_err_b.
-     pose proof (nth_error_value_length _ _ _ _ nth_err_b).
-     rewrite base_from_limb_widths_length in *.
-     rewrite nth_error_base in nth_err_b by assumption.
-     rewrite two_p_correct in nth_err_b.
-     congruence.
-   Qed.
-
-   Lemma base_positive : forall b : Z, In b base -> b > 0.
-   Proof using Type*.
-     intros b In_b_base.
-     apply In_nth_error_value in In_b_base.
-     destruct In_b_base as [i nth_err_b].
-     apply nth_error_subst in nth_err_b.
-     rewrite nth_err_b.
-     apply Z.gt_lt_iff.
-     apply Z.pow_pos_nonneg; omega || auto using sum_firstn_limb_widths_nonneg.
-   Qed.
-
    Lemma b0_1 : forall x : Z, limb_widths <> nil -> nth_default x base 0 = 1.
    Proof using Type.
      case_eq limb_widths; intros; [congruence | reflexivity].
@@ -229,27 +180,6 @@ Section Pow2BaseProofs.
     apply nth_default_preserves_properties; auto; omega.
   Qed.
 
-  Lemma pow2_mod_bounded_iff :forall lw us, (forall w, In w lw -> 0 <= w) -> (bounded lw us <->
-    (forall i, Z.pow2_mod (nth_default 0 us i) (nth_default 0 lw i) = nth_default 0 us i)).
-  Proof using Type.
-    clear.
-    split; intros; auto using pow2_mod_bounded.
-    cbv [bounded]; intros.
-    assert (0 <= nth_default 0 lw i) by (apply nth_default_preserves_properties; auto; omega).
-    split.
-    + specialize (H0 i).
-      rewrite Z.pow2_mod_spec in H0 by assumption.
-      apply Z.mod_small_iff in H0; [ | apply Z.pow_nonzero; (assumption || omega)].
-      destruct H0; try omega.
-      pose proof (Z.pow_nonneg 2 (nth_default 0 lw i)).
-      specialize_by omega; omega.
-    + apply Z.testbit_false_bound; auto.
-      intros.
-      rewrite <-H0.
-      rewrite Z.testbit_pow2_mod by assumption.
-      break_if; reflexivity || omega.
-  Qed.
-
   Lemma bounded_nil_iff : forall us, bounded nil us <-> (forall u, In u us -> u = 0).
   Proof using Type.
     clear.
@@ -277,7 +207,7 @@ Section Pow2BaseProofs.
                                     nth_default 0 us i = Z.pow2_mod (BaseSystem.decode base us >> sum_firstn limb_widths i) (nth_default 0 limb_widths i).
   Proof using Type*.
     intro; revert limb_widths limb_widths_nonneg; induction us; intros.
-    + rewrite nth_default_nil, decode_nil, Z.shiftr_0_l, Z.pow2_mod_spec, Z.mod_0_l by
+    + rewrite nth_default_nil, BaseSystemProofs.decode_nil, Z.shiftr_0_l, Z.pow2_mod_spec, Z.mod_0_l by
           (try (apply Z.pow_nonzero; try omega); apply nth_default_preserves_properties; auto; omega).
       reflexivity.
     + destruct i.
@@ -286,11 +216,11 @@ Section Pow2BaseProofs.
         * cbv [base_from_limb_widths].
           rewrite <-pow2_mod_bounded with (lw := nil); rewrite bounded_nil_iff in *; auto using in_cons;
             try solve [intros; exfalso; eauto using in_nil].
-          rewrite !nth_default_nil, decode_base_nil; auto.
+          rewrite !nth_default_nil, BaseSystemProofs.decode_base_nil; auto.
           cbv. auto using in_eq.
-        * rewrite nth_default_cons, base_from_limb_widths_cons, peel_decode.
+        * rewrite nth_default_cons, base_from_limb_widths_cons, BaseSystemProofs.peel_decode.
           fold (BaseSystem.mul_each (two_p w)).
-          rewrite <-mul_each_base, mul_each_rep.
+          rewrite <-BaseSystemProofs.mul_each_base, BaseSystemProofs.mul_each_rep.
           rewrite two_p_correct, (Z.mul_comm (2 ^ w)).
           rewrite <-Z.shiftl_mul_pow2 by auto using in_eq.
           rewrite bounded_iff in *.
@@ -311,12 +241,12 @@ Section Pow2BaseProofs.
         destruct limb_widths as [|w lw].
         * cbv [base_from_limb_widths].
           rewrite <-pow2_mod_bounded with (lw := nil); rewrite bounded_nil_iff in *; auto using in_cons.
-          rewrite sum_firstn_nil, !nth_default_nil, decode_base_nil, Z.shiftr_0_r.
+          rewrite sum_firstn_nil, !nth_default_nil, BaseSystemProofs.decode_base_nil, Z.shiftr_0_r.
           apply nth_default_preserves_properties; intros; auto using in_cons.
           f_equal; auto using in_cons.
-        * rewrite sum_firstn_succ_cons, nth_default_cons_S, base_from_limb_widths_cons, peel_decode.
+        * rewrite sum_firstn_succ_cons, nth_default_cons_S, base_from_limb_widths_cons, BaseSystemProofs.peel_decode.
           fold (BaseSystem.mul_each (two_p w)).
-          rewrite <-mul_each_base, mul_each_rep.
+          rewrite <-BaseSystemProofs.mul_each_base, BaseSystemProofs.mul_each_rep.
           rewrite two_p_correct, (Z.mul_comm (2 ^ w)).
           rewrite <-Z.shiftl_mul_pow2 by auto using in_eq.
           rewrite bounded_iff in *.
@@ -334,22 +264,6 @@ Section Pow2BaseProofs.
     intros; apply nth_default_preserves_properties; auto; omega.
   Qed. Hint Resolve nth_default_limb_widths_nonneg.
 
-  Lemma parity_decode : forall x,
-    (0 < nth_default 0 limb_widths 0) ->
-    length x = length limb_widths ->
-    Z.odd (BaseSystem.decode base x) = Z.odd (nth_default 0 x 0).
-  Proof using Type*.
-    intros.
-    destruct limb_widths, x; simpl in *; try discriminate; try reflexivity.
-    rewrite peel_decode, nth_default_cons.
-    fold (BaseSystem.mul_each (two_p z)).
-    rewrite <-mul_each_base, mul_each_rep.
-    rewrite Z.odd_add_mul_even; [ f_equal; ring | ].
-    rewrite <-Z.even_spec, two_p_correct.
-    apply Z.even_pow.
-    rewrite @nth_default_cons in *; auto.
-  Qed.
-
   Lemma decode_firstn_pow2_mod : forall us i,
     (i <= length us)%nat ->
     length us = length limb_widths ->
@@ -358,11 +272,11 @@ Section Pow2BaseProofs.
   Proof using Type*.
     intros; induction i;
     repeat match goal with
-           | |- _ => rewrite sum_firstn_0, decode_nil, Z.pow2_mod_0_r; reflexivity
+           | |- _ => rewrite sum_firstn_0, BaseSystemProofs.decode_nil, Z.pow2_mod_0_r; reflexivity
            | |- _ => progress distr_length
            | |- _ => progress autorewrite with simpl_firstn
            | |- _ => rewrite firstn_succ with (d := 0)
-           | |- _ => rewrite set_higher
+           | |- _ => rewrite BaseSystemProofs.set_higher
            | |- _ => rewrite nth_default_base
            | |- _ => rewrite IHi
            | |- _ => rewrite <-Z.lor_shiftl by (rewrite ?Z.pow2_mod_spec; try apply Z.mod_pos_bound; zero_bounds)
@@ -459,82 +373,15 @@ Section Pow2BaseProofs.
         replace (length us) with (length limb_widths); try omega. }
   Qed.
 
-  Lemma decode_firstn_succ : forall us i,
-      (S i <= length us)%nat ->
-      bounded limb_widths us ->
-      length us = length limb_widths ->
-      BaseSystem.decode base (firstn (S i) us) =
-      Z.lor (BaseSystem.decode base (firstn i us)) (nth_default 0 us i << sum_firstn limb_widths i).
-  Proof using Type*.
-    repeat match goal with
-           | |- _ => progress intros
-           | |- _ => progress autorewrite with Ztestbit
-           | |- _ => progress change BaseSystem.decode with BaseSystem.decode'
-           | |- _ => rewrite sum_firstn_succ_default in *
-           | |- _ => apply Z.bits_inj'
-           | |- _ => break_if
-           | |- appcontext [Z.testbit _ (?a - sum_firstn ?l ?i)] =>
-                  destruct (Z_le_dec (sum_firstn l i) a);
-                  [ rewrite (testbit_decode_firstn_high _ i a)
-                  | rewrite (Z.testbit_neg_r _ (a - sum_firstn l i))]
-           | |- appcontext [Z.testbit (BaseSystem.decode' _ (firstn ?i _)) _] =>
-                  rewrite (decode_firstn_pow2_mod _ i)
-           | |- _ => rewrite digit_select by auto
-           | |- _ => rewrite Z.testbit_pow2_mod
-           | |- _ => assumption
-           | |- _ => reflexivity
-           | |- _ => omega
-           | |- _ => f_equal; ring
-           | |- _ => solve [auto]
-           | |- _ => solve [zero_bounds]
-           | H : appcontext [nth_default 0 limb_widths ?i] |- _ =>
-             pose proof (nth_default_limb_widths_nonneg i); omega
-           | |- appcontext [nth_default 0 limb_widths ?i] =>
-             pose proof (nth_default_limb_widths_nonneg i); omega
-           end.
-  Qed.
-
-  Lemma testbit_decode_digit_select : forall us n i,
-    bounded limb_widths us ->
-    sum_firstn limb_widths i <= n < sum_firstn limb_widths (S i) ->
-    Z.testbit (BaseSystem.decode base us) n = Z.testbit (nth_default 0 us i) (n - sum_firstn limb_widths i).
-  Proof using Type*.
-    repeat match goal with
-           | |- _ => progress intros
-           | |- _ => erewrite digit_select by eauto
-           | |- _ => progress rewrite sum_firstn_succ_default in *
-           | |- _ => progress autorewrite with Ztestbit
-           | |- _ => break_if
-           | |- _ => omega
-           | |- _ => solve [f_equal;ring]
-           end.
-  Qed.
-
-  Lemma testbit_bounded_high : forall i n us, bounded limb_widths us ->
-                                            nth_default 0 limb_widths i <= n ->
-                                            Z.testbit (nth_default 0 us i) n = false.
-  Proof using Type*.
-    repeat match goal with
-           | |- _ => progress intros
-           | |- _ => break_if
-           | |- _ => omega
-           | |- _ => reflexivity
-           | |- _ => assumption
-           | |- _ => apply nth_default_limb_widths_nonneg; auto
-           | H : nth_default 0 limb_widths ?i <= ?n |- 0 <= ?n => etransitivity; [ | eapply H]
-           | |- _ => erewrite <-pow2_mod_bounded by eauto; rewrite Z.testbit_pow2_mod
-           end.
-  Qed.
-
   Lemma decode_shift_app : forall us0 us1, (length (us0 ++ us1) <= length limb_widths)%nat ->
     BaseSystem.decode base (us0 ++ us1) = (BaseSystem.decode (base_from_limb_widths (firstn (length us0) limb_widths)) us0) + ((BaseSystem.decode (base_from_limb_widths (skipn (length us0) limb_widths)) us1) << sum_firstn limb_widths (length us0)).
   Proof using Type*.
     unfold BaseSystem.decode; intros us0 us1 ?.
     assert (0 <= sum_firstn limb_widths (length us0)) by auto using sum_firstn_nonnegative.
-    rewrite decode'_splice; autorewrite with push_firstn.
+    rewrite BaseSystemProofs.decode'_splice; autorewrite with push_firstn.
     apply Z.add_cancel_l.
     autorewrite with pull_base_from_limb_widths Zshift_to_pow zsimplify.
-    rewrite decode'_map_mul, two_p_correct; nia.
+    rewrite BaseSystemProofs.decode'_map_mul, two_p_correct; nia.
   Qed.
 
   Lemma decode_shift : forall us u0, (length (u0 :: us) <= length limb_widths)%nat ->
@@ -564,72 +411,6 @@ Section Pow2BaseProofs.
     reflexivity.
   Qed.
 
-  Lemma bounded_nil_r : forall l, (forall x, In x l -> 0 <= x) -> bounded l nil.
-  Proof using Type.
-    cbv [bounded]; intros.
-    rewrite nth_default_nil.
-    apply nth_default_preserves_properties; intros; split; zero_bounds.
-  Qed.
-
-  Section make_base_vector.
-    Local Notation k := (sum_firstn limb_widths (length limb_widths)).
-    Context (limb_widths_match_modulus : forall i j,
-                (i < length base)%nat ->
-                (j < length base)%nat ->
-                (i + j >= length base)%nat ->
-                let w_sum := sum_firstn limb_widths in
-                k + w_sum (i + j - length base)%nat <= w_sum i + w_sum j)
-            (limb_widths_good : forall i j, (i + j < length limb_widths)%nat ->
-                                            sum_firstn limb_widths (i + j) <=
-                                            sum_firstn limb_widths i + sum_firstn limb_widths j).
-
-    Lemma base_matches_modulus: forall i j,
-      (i   <  length base)%nat ->
-      (j   <  length base)%nat ->
-      (i+j >= length base)%nat->
-      let b := nth_default 0 base in
-      let r := (b i * b j)  /   (2^k * b (i+j-length base)%nat) in
-                b i * b j = r * (2^k * b (i+j-length base)%nat).
-    Proof using limb_widths_match_modulus limb_widths_nonneg.
-      intros.
-      rewrite (Z.mul_comm r).
-      subst r.
-      rewrite base_from_limb_widths_length in *;
-      assert (i + j - length limb_widths < length limb_widths)%nat by omega.
-      rewrite Z.mul_div_eq by (apply Z.gt_lt_iff; subst b; rewrite ?nth_default_base; zero_bounds;
-        assumption).
-      rewrite (Zminus_0_l_reverse (b i * b j)) at 1.
-      f_equal.
-      subst b.
-      repeat rewrite nth_default_base by auto.
-      do 2 rewrite <- Z.pow_add_r by auto using sum_firstn_limb_widths_nonneg.
-      symmetry.
-      apply Z.mod_same_pow.
-      split.
-      + apply Z.add_nonneg_nonneg; auto using sum_firstn_limb_widths_nonneg.
-      + auto using limb_widths_match_modulus.
-    Qed.
-
-    Lemma base_good : forall i j : nat,
-                 (i + j < length base)%nat ->
-                 let b := nth_default 0 base in
-                 let r := b i * b j / b (i + j)%nat in
-                 b i * b j = r * b (i + j)%nat.
-    Proof using limb_widths_good limb_widths_nonneg.
-      intros; subst b r.
-      clear limb_widths_match_modulus.
-      rewrite base_from_limb_widths_length in *.
-      repeat rewrite nth_default_base by omega.
-      rewrite (Z.mul_comm _ (2 ^ (sum_firstn limb_widths (i+j)))).
-      rewrite Z.mul_div_eq by (apply Z.gt_lt_iff; zero_bounds;
-        auto using sum_firstn_limb_widths_nonneg).
-      rewrite <- Z.pow_add_r by auto using sum_firstn_limb_widths_nonneg.
-      rewrite Z.mod_same_pow; try ring.
-      split; [ auto using sum_firstn_limb_widths_nonneg | ].
-      apply limb_widths_good.
-      assumption.
-    Qed.
-  End make_base_vector.
 End Pow2BaseProofs.
 Hint Rewrite base_from_limb_widths_cons base_from_limb_widths_nil : push_base_from_limb_widths.
 Hint Rewrite <- base_from_limb_widths_cons : pull_base_from_limb_widths.
@@ -646,184 +427,6 @@ Hint Rewrite @skipn_base_from_limb_widths : push_skipn.
 Hint Rewrite @base_from_limb_widths_length : distr_length.
 Hint Rewrite @upper_bound_nil @upper_bound_cons @upper_bound_app using solve [ eauto with znonzero ] : push_upper_bound.
 Hint Rewrite <- @upper_bound_cons @upper_bound_app using solve [ eauto with znonzero ] : pull_upper_bound.
-
-Section BitwiseDecodeEncode.
-  Context {limb_widths} (limb_widths_nonnil : limb_widths <> nil)
-          (limb_widths_nonneg : forall w, In w limb_widths -> 0 <= w)
-          (limb_widths_good : forall i j, (i + j < length limb_widths)%nat ->
-                                          sum_firstn limb_widths (i + j) <=
-                                          sum_firstn limb_widths i + sum_firstn limb_widths j).
-  Local Hint Resolve limb_widths_nonneg.
-  Local Hint Resolve nth_default_limb_widths_nonneg.
-  Local Hint Resolve sum_firstn_limb_widths_nonneg.
-  Local Notation "w[ i ]" := (nth_default 0 limb_widths i).
-  Local Notation base := (base_from_limb_widths limb_widths).
-  Local Notation upper_bound := (upper_bound limb_widths).
-
-  Lemma encode'_spec : forall x i, (i <= length limb_widths)%nat ->
-    encode' limb_widths x i = BaseSystem.encode' base x upper_bound i.
-  Proof using limb_widths_nonneg.
-    induction i; intros.
-    + rewrite encode'_zero. reflexivity.
-    + rewrite encode'_succ, <-IHi by omega.
-      simpl; do 2 f_equal.
-      rewrite Z.land_ones, Z.shiftr_div_pow2 by auto.
-      match goal with H : (S _ <= length limb_widths)%nat |- _ =>
-        apply le_lt_or_eq in H; destruct H end.
-      - repeat f_equal; rewrite nth_default_base by (omega || auto); reflexivity.
-      - repeat f_equal; try solve [rewrite nth_default_base by (omega || auto); reflexivity].
-        rewrite nth_default_out_of_bounds by (distr_length; omega).
-        unfold Pow2Base.upper_bound.
-        congruence.
-  Qed.
-
-  Lemma length_encode' : forall lw z i, length (encode' lw z i) = i.
-  Proof using Type.
-    induction i; intros; simpl encode'; distr_length.
-  Qed.
-  Hint Rewrite length_encode' : distr_length.
-
-  Lemma bounded_encode' : forall z i, (0 <= z) ->
-    bounded (firstn i limb_widths) (encode' limb_widths z i).
-  Proof using limb_widths_nonneg.
-    intros; induction i; simpl encode';
-      repeat match goal with
-             | |- _ => progress intros
-             | |- _ => progress autorewrite with push_nth_default in *
-             | |- _ => progress autorewrite with Ztestbit
-             | |- _ => progress rewrite ?firstn_O, ?Nat.sub_diag in *
-             | |- _ => rewrite Z.testbit_pow2_mod by auto
-             | |- _ => rewrite Z.ones_spec by zero_bounds
-             | |- _ => rewrite sum_firstn_succ_default
-             | |- _ => rewrite nth_default_out_of_bounds by distr_length
-             | |- _ => break_if; distr_length
-             | |- _ => apply bounded_nil_r
-             | |- appcontext[nth_default _ (_ :: nil) ?i] => case_eq i; intros; autorewrite with push_nth_default
-             | |- Z.pow2_mod (?a >> ?b) _ = (?a >> ?b) => apply Z.bits_inj'
-             | IH : forall i, _ = nth_default 0 (encode' _ _ _) i
-                              |- appcontext[nth_default 0 limb_widths ?i] => specialize (IH i)
-             | H : In _ (firstn _ _) |- _ => apply In_firstn in H
-             | H1 : ~ (?a < ?b)%nat, H2 : (?a < S ?b)%nat |- _ =>
-               progress replace a with b in * by omega
-             | H : bounded _ _ |- bounded _ _ =>
-               apply pow2_mod_bounded_iff; rewrite pow2_mod_bounded_iff in H
-             | |- _ => solve [auto]
-             | |- _ => contradiction
-             | |- _ => reflexivity
-             end.
-  Qed.
-
-  Lemma bounded_encodeZ : forall z, (0 <= z) ->
-    bounded limb_widths (encodeZ limb_widths z).
-  Proof using limb_widths_nonneg.
-    cbv [encodeZ]; intros.
-    pose proof (bounded_encode' z (length limb_widths)) as Hencode'.
-    rewrite firstn_all in Hencode'; auto.
-  Qed.
-
-  Lemma base_upper_bound_compatible : @base_max_succ_divide base upper_bound.
-  Proof using limb_widths_nonneg.
-    unfold base_max_succ_divide; intros i lt_Si_length.
-    rewrite base_from_limb_widths_length in lt_Si_length.
-    rewrite Nat.lt_eq_cases in lt_Si_length; destruct lt_Si_length;
-      rewrite !nth_default_base by (omega || auto).
-    + erewrite sum_firstn_succ by (eapply nth_error_Some_nth_default with (x := 0); omega).
-      rewrite Z.pow_add_r; eauto.
-      apply Z.divide_factor_r.
-    + rewrite nth_default_out_of_bounds by (distr_length; omega).
-      unfold Pow2Base.upper_bound.
-      replace (length limb_widths) with (S (pred (length limb_widths))) by omega.
-      replace i with (pred (length limb_widths)) by omega.
-      erewrite sum_firstn_succ by (eapply nth_error_Some_nth_default with (x := 0); omega).
-      rewrite Z.pow_add_r; eauto.
-      apply Z.divide_factor_r.
-  Qed.
-  Hint Resolve base_upper_bound_compatible.
-
-  Lemma encodeZ_spec : forall x,
-    BaseSystem.decode base (encodeZ limb_widths x) = x mod upper_bound.
-  Proof.
-    intros.
-    assert (length base = length limb_widths) by distr_length.
-    unfold encodeZ; rewrite encode'_spec by omega.
-    erewrite BaseSystemProofs.encode'_spec; unfold Pow2Base.upper_bound;
-      zero_bounds; intros; eauto using base_positive, b0_1. {
-      rewrite nth_default_out_of_bounds by omega.
-      reflexivity.
-    } {
-      econstructor; try apply base_good;
-        eauto using base_positive, b0_1.
-    }
-  Qed.
-
-  Lemma encodeZ_length : forall x, length (encodeZ limb_widths x) = length limb_widths.
-  Proof using limb_widths_nonneg.
-    cbv [encodeZ]; intros.
-    rewrite encode'_spec by omega.
-    apply encode'_length.
-  Qed.
-
-  Definition decode_bitwise'_invariant us i acc :=
-    forall n, 0 <= n -> Z.testbit acc n = Z.testbit (BaseSystem.decode base us) (n + sum_firstn limb_widths i).
-
-  Lemma decode_bitwise'_invariant_step : forall us,
-    length us = length limb_widths ->
-    bounded limb_widths us ->
-    forall i acc, decode_bitwise'_invariant us (S i) acc ->
-                  decode_bitwise'_invariant us i (Z.lor (nth_default 0 us i) (acc << nth_default 0 limb_widths i)).
-  Proof using limb_widths_nonneg.
-    repeat match goal with
-      | |- _ => progress cbv [decode_bitwise'_invariant]; intros
-      | |- _ => erewrite testbit_bounded_high by (omega || eauto)
-      | |- _ => progress autorewrite with Ztestbit
-      | |- _ => progress rewrite sum_firstn_succ_default
-      | |- appcontext[Z.testbit _ ?n] => rewrite (Z.testbit_neg_r _ n) by omega
-      | H : forall n, 0 <= n -> Z.testbit _ n = _ |- _ => rewrite H by omega
-      | |- _ => solve [f_equal; ring]
-      | |- appcontext[Z.testbit _ (?x + sum_firstn limb_widths ?i)] =>
-        erewrite testbit_decode_digit_select with (i0 := i) by
-          (eauto; rewrite sum_firstn_succ_default; omega)
-      | |- appcontext[Z.testbit _ (?a - ?b)] => destruct (Z_lt_dec a b)
-      | _ => progress break_if
-      end.
-  Qed.
-
-  Lemma decode_bitwise'_invariant_holds : forall i us acc,
-    length us = length limb_widths ->
-    bounded limb_widths us ->
-    decode_bitwise'_invariant us i acc ->
-    decode_bitwise'_invariant us 0 (decode_bitwise' limb_widths us i acc).
-  Proof using limb_widths_nonneg.
-    repeat match goal with
-           | |- _ => progress intros
-           | |- _ => solve [auto using decode_bitwise'_invariant_step]
-           | |- appcontext[decode_bitwise' ?a ?b ?c ?d] =>
-                functional induction (decode_bitwise' a b c d)
-            end.
-  Qed.
-
-  Lemma decode_bitwise_spec : forall us, bounded limb_widths us ->
-    length us = length limb_widths ->
-    decode_bitwise limb_widths us = BaseSystem.decode base us.
-  Proof using limb_widths_nonneg.
-    repeat match goal with
-           | |- _ => progress cbv [decode_bitwise decode_bitwise'_invariant] in *
-           | |- _ => progress intros
-           | |- _ => rewrite sum_firstn_0
-           | |- _ => erewrite testbit_decode_high by (assumption || omega)
-           | H0 : ?P ?x , H1 : ?P ?x -> _ |- _ => specialize (H1 H0)
-           | H : _ -> forall n, 0 <= n -> Z.testbit _ n = _ |- _ => rewrite H
-           | |- decode_bitwise' ?a ?b ?c ?d = _ =>
-                  let H := fresh "H" in
-                  pose proof (decode_bitwise'_invariant_holds c b d) as H;
-                    apply Z.bits_inj'
-           | |- _ => apply Z.testbit_0_l
-           | |- _ => assumption
-           | |- _ => solve [f_equal; ring]
-           end.
-  Qed.
-
-End BitwiseDecodeEncode.
 
 Section UniformBase.
   Context {width : Z} (limb_width_nonneg : 0 <= width).
@@ -900,11 +503,11 @@ Section UniformBase.
   Proof using Type.
     clear.
     induction us; intros.
-    + rewrite !decode_nil; reflexivity.
+    + rewrite !BaseSystemProofs.decode_nil; reflexivity.
     + distr_length.
       destruct bs.
-      - rewrite firstn_nil, !decode_base_nil; reflexivity.
-      - rewrite firstn_cons, !peel_decode.
+      - rewrite firstn_nil, !BaseSystemProofs.decode_base_nil; reflexivity.
+      - rewrite firstn_cons, !BaseSystemProofs.peel_decode.
         f_equal.
         apply IHus.
   Qed.
@@ -949,609 +552,4 @@ Section UniformBase.
     rewrite decode_shift_app by auto using uniform_limb_widths_nonneg.
     reflexivity.
   Qed.
-
-  Lemma decode_shift_uniform : forall us u0, (length (u0 :: us) <= length limb_widths)%nat ->
-    BaseSystem.decode base (u0 :: us) = u0 + ((BaseSystem.decode base us) << width).
-  Proof using Type*.
-    intros.
-    rewrite decode_tl_base with (us := us) by distr_length.
-    apply decode_shift_uniform_tl; assumption.
-  Qed.
-
 End UniformBase.
-
-Hint Rewrite @upper_bound_uniform using solve [ auto with datatypes ] : push_upper_bound.
-
-Section SplitIndex.
-  (* This section defines [split_index], which for a list of bounded digits
-       splits a bit index in the decoded value into a digit index and a bit
-       index within the digit. Examples:
-       limb_widths [4;4] : split_index 6 = (1,2)
-       limb_widths [26,25,26] : split_index 30 = (1,4)
-       limb_widths [26,25,26] : split_index 51 = (2,0)
-  *)
-  Local Notation "u # i" := (nth_default 0 u i).
-
-  Function split_index' i index lw :=
-    match lw with
-    | nil      => (index, i)
-    | w :: lw' => if Z_lt_dec i w then (index, i)
-                  else split_index' (i - w) (S index) lw'
-    end.
-
-  Lemma split_index'_ge_index : forall i index lw, (index <= fst (split_index' i index lw))%nat.
-  Proof.
-    intros; functional induction (split_index' i index lw);
-      repeat match goal with
-             | |- _ => omega
-             | |- _ => progress (simpl fst; simpl snd)
-             end.
-  Qed.
-
-  Lemma split_index'_done_case : forall i index lw, 0 <= i ->
-                                                    (forall x, In x lw -> 0 <= x) ->
-    if Z_lt_dec i (sum_firstn lw (length lw))
-    then (fst (split_index' i index lw) - index < length lw)%nat
-    else (fst (split_index' i index lw) - index = length lw)%nat.
-  Proof.
-    intros; functional induction (split_index' i index lw);
-      repeat match goal with
-             | |- _ => break_if
-             | |- _ => rewrite sum_firstn_nil in *
-             | |- _ => rewrite sum_firstn_succ_cons in *
-             | |- _ => progress distr_length
-             | |- _ => progress (simpl fst; simpl snd)
-             | H : appcontext [split_index' ?a ?b ?c] |- _ =>
-               unique pose proof (split_index'_ge_index a b c)
-             | H : appcontext [sum_firstn ?l ?i] |- _ =>
-               let H0 := fresh "H" in
-               assert (forall x, In x l -> 0 <= x) by auto using in_cons;
-               unique pose proof (sum_firstn_limb_widths_nonneg H0 i)
-             | |- _ => progress specialize_by assumption
-             | |- _ => progress specialize_by omega
-             | |- _ => omega
-             end.
-  Qed.
-
-  Lemma snd_split_index'_nonneg : forall index lw i, (0 <= i) ->
-                                                     (0 <= snd (split_index' i index lw)).
-  Proof.
-    intros; functional induction (split_index' i index lw);
-      repeat match goal with
-             | |- _ => omega
-             | H : ?P -> ?G |- ?G => apply H
-             | |- _ => progress (simpl fst; simpl snd)
-             end.
-  Qed.
-
-  Lemma snd_split_index'_small : forall i index lw, 0 <= i < sum_firstn lw (length lw) ->
-      (snd (split_index' i index lw) < lw # (fst (split_index' i index lw) - index)).
-  Proof.
-    intros; functional induction (split_index' i index lw);
-      try match goal with |- appcontext [split_index' ?a ?b ?c] =>
-                    pose proof (split_index'_ge_index a b c) end;
-      repeat match goal with
-             | |- _ => progress autorewrite with push_nth_default distr_length in *
-             | |- _ => rewrite Nat.sub_diag
-             | |- _ => rewrite sum_firstn_nil in *
-             | |- _ => rewrite sum_firstn_succ_cons in *
-             | |- _ => progress (simpl fst; simpl snd)
-             | H : _ -> ?x < _ |- ?x < _ => eapply Z.lt_le_trans; [ apply H; omega | ]
-             | |- ?xs # (?a - S ?b) <= (_ :: ?xs) # (?a - ?b) =>
-               replace (a - b)%nat with (S (a - S b))%nat
-             | |- _ => omega
-             end.
-  Qed.
-
-  Lemma split_index'_correct : forall i index lw,
-    sum_firstn lw (fst (split_index' i index lw) - index) + (snd (split_index' i index lw)) = i.
-  Proof.
-    intros; functional induction (split_index' i index lw);
-      repeat match goal with
-             | |- _ => omega
-             | |- _ => rewrite Nat.sub_diag
-             | |- _ => progress rewrite ?sum_firstn_nil, ?sum_firstn_0, ?sum_firstn_succ_cons
-             | |- _ => progress (simpl fst; simpl snd)
-             | |- appcontext[(fst (split_index' ?i (S ?idx) ?lw) - ?idx)%nat] =>
-               pose proof (split_index'_ge_index i (S idx) lw);
-                 replace (fst (split_index' i (S idx) lw) - idx)%nat with
-                   (S (fst (split_index' i (S idx) lw) - S idx))%nat
-             end.
-  Qed.
-
-  Context limb_widths
-          (limb_widths_pos : forall w, In w limb_widths -> 0 <= w).
-  Local Hint Resolve limb_widths_pos.
-  Local Notation base := (base_from_limb_widths limb_widths).
-  Local Notation bitsIn lw := (sum_firstn lw (length lw)).
-
-  Definition split_index i := split_index' i 0 limb_widths.
-  Definition digit_index i := fst (split_index i).
-  Definition bit_index i := snd (split_index i).
-
-  Lemma testbit_decode : forall us n,
-    0 <= n < bitsIn limb_widths ->
-    length us = length limb_widths ->
-    bounded limb_widths us ->
-    Z.testbit (BaseSystem.decode base us) n = Z.testbit (us # digit_index n) (bit_index n).
-  Proof using Type*.
-    cbv [digit_index bit_index split_index]; intros.
-    pose proof (split_index'_correct n 0 limb_widths).
-    pose proof (snd_split_index'_nonneg 0 limb_widths n).
-    specialize_by assumption.
-    repeat match goal with
-           | |- _ => progress autorewrite with Ztestbit natsimplify in *
-           | |- _ => erewrite digit_select by eauto
-           | |- _ => break_if
-           | |- _ => rewrite Z.testbit_pow2_mod by auto using nth_default_limb_widths_nonneg
-           | |- _ => omega
-           | |- _ => f_equal; omega
-           end.
-    destruct (Z_lt_dec n (bitsIn limb_widths)). {
-      pose proof (snd_split_index'_small n 0 limb_widths).
-      specialize_by omega.
-      rewrite Nat.sub_0_r in *.
-      omega.
-    } {
-      apply testbit_decode_high; auto.
-      replace (length us) with (length limb_widths) in *.
-      omega.
-    }
-  Qed.
-
-  Lemma testbit_decode_full : forall us n,
-    length us = length limb_widths ->
-    bounded limb_widths us ->
-    Z.testbit (BaseSystem.decode base us) n =
-    if Z_le_dec 0 n
-    then (if Z_lt_dec n (bitsIn limb_widths)
-          then Z.testbit (us # digit_index n) (bit_index n)
-          else false)
-    else false.
-  Proof using Type*.
-    repeat match goal with
-           | |- _ => progress intros
-           | |- _ => break_if
-           | |- _ => apply Z.testbit_neg_r; lia
-           | |- _ => apply testbit_decode_high; auto;
-                       try match goal with H : length _ = length limb_widths |- _ => rewrite H end; lia
-           | |- _ => auto using testbit_decode
-           end.
-  Qed.
-
-  Lemma bit_index_nonneg : forall i, 0 <= i -> 0 <= bit_index i.
-  Proof using Type.
-    apply snd_split_index'_nonneg.
-  Qed.
-
-  Lemma digit_index_lt_length : forall i, 0 <= i < bitsIn limb_widths ->
-                                         (digit_index i < length limb_widths)%nat.
-  Proof using Type*.
-    cbv [bit_index digit_index split_index]; intros.
-    pose proof (split_index'_done_case i 0 limb_widths).
-    specialize_by lia. specialize_by eauto.
-    break_if; lia.
-  Qed.
-
-  Lemma bit_index_not_done : forall i, 0 <= i < bitsIn limb_widths ->
-                                         (bit_index i < limb_widths # digit_index i).
-  Proof using Type.
-
-    cbv [bit_index digit_index split_index]; intros.
-    eapply Z.lt_le_trans; try apply (snd_split_index'_small i 0 limb_widths); try assumption.
-    rewrite Nat.sub_0_r; lia.
-  Qed.
-
-  Lemma split_index_eqn : forall i, 0 <= i < bitsIn limb_widths ->
-    sum_firstn limb_widths (digit_index i) + bit_index i = i.
-  Proof using Type.
-    cbv [bit_index digit_index split_index]; intros.
-    etransitivity;[ | apply (split_index'_correct i 0 limb_widths) ].
-    repeat f_equal; omega.
-  Qed.
-
-  Lemma rem_bits_in_digit_pos : forall i, 0 <= i < bitsIn limb_widths ->
-                                          0 < (limb_widths # digit_index i) - bit_index i.
-  Proof using Type.
-    repeat match goal with
-           | |- _ => progress intros
-           | |- 0 < ?a - ?b => destruct (Z_lt_dec b a); [ lia | exfalso ]
-           | H : ~ (bit_index ?i < limb_widths # digit_index ?i) |- _ =>
-             pose proof (bit_index_not_done i); specialize_by omega; omega
-           end.
-  Qed.
-
-
-  Lemma rem_bits_in_digit_le_rem_bits : forall i, 0 <= i < bitsIn limb_widths ->
-                                                    i + ((limb_widths # digit_index i) - bit_index i) <= bitsIn limb_widths.
-  Proof using Type*.
-    intros.
-    rewrite <-(split_index_eqn i) at 1 by lia.
-    match goal with
-    | |- ?a + ?b + (?c - ?b) <= _ => replace (a + b + (c - b)) with (c + a) by ring
-    end.
-    rewrite <-sum_firstn_succ_default.
-    apply sum_firstn_prefix_le; auto.
-    pose proof (digit_index_lt_length i H); lia.
-  Qed.
-
-
-  Lemma same_digit : forall i j, 0 <= i <= j ->
-                                 j < bitsIn limb_widths ->
-                                 j < i + ((limb_widths # (digit_index i)) - bit_index i) ->
-                                 (digit_index i = digit_index j)%nat.
-  Proof using Type*.
-    intros.
-    pose proof (split_index_eqn i).
-    pose proof (split_index_eqn j).
-    specialize_by lia.
-    apply le_antisym. {
-      eapply sum_firstn_pos_lt_succ; eauto; try (apply digit_index_lt_length; auto; lia).
-      rewrite sum_firstn_succ_default.
-      eapply Z.le_lt_trans; [ | apply Z.add_lt_mono_r; apply bit_index_not_done; lia ].
-      pose proof (bit_index_nonneg i).
-      specialize_by lia.
-      lia.
-    } {
-      eapply sum_firstn_pos_lt_succ; eauto; try (apply digit_index_lt_length; auto; lia).
-      rewrite <-H2 in H1 at 1.
-      match goal with
-      | H : _ < ?a + ?b + (?c - ?b) |- _ => replace (a + b + (c - b)) with (c + a) in H by ring;
-                                              rewrite <-sum_firstn_succ_default in H
-      end.
-      rewrite <-H3 in H1.
-      pose proof (bit_index_nonneg j). specialize_by lia.
-      lia.
-    }
-  Qed.
-
-  Lemma same_digit_bit_index_sub : forall i j, 0 <= i <= j -> j < bitsIn limb_widths ->
-                                               digit_index i = digit_index j ->
-                                               bit_index j - bit_index i = j - i.
-  Proof using Type.
-    intros.
-    pose proof (split_index_eqn i).
-    pose proof (split_index_eqn j).
-    specialize_by lia.
-    rewrite H1 in *.
-    lia.
-  Qed.
-
-End SplitIndex.
-
-Section carrying_helper.
-  Context {limb_widths} (limb_widths_nonneg : forall w, In w limb_widths -> 0 <= w).
-  Local Notation base := (base_from_limb_widths limb_widths).
-  Local Notation log_cap i := (nth_default 0 limb_widths i).
-
-  Lemma update_nth_sum : forall n f us, (n < length us \/ n >= length limb_widths)%nat ->
-    BaseSystem.decode base (update_nth n f us) =
-    (let v := nth_default 0 us n in f v - v) * nth_default 0 base n + BaseSystem.decode base us.
-  Proof using Type.
-    intros.
-    unfold BaseSystem.decode.
-    destruct H as [H|H].
-    { nth_inbounds; auto. (* TODO(andreser): nth_inbounds should do this auto*)
-      erewrite nth_error_value_eq_nth_default by eassumption.
-      unfold splice_nth.
-      rewrite <- (firstn_skipn n us) at 3.
-      do 2 rewrite decode'_splice.
-      remember (length (firstn n us)) as n0.
-      ring_simplify.
-      remember (BaseSystem.decode' (firstn n0 base) (firstn n us)).
-      rewrite (skipn_nth_default n us 0) by omega.
-      erewrite (nth_error_value_eq_nth_default _ _ us) by eassumption.
-      rewrite firstn_length in Heqn0.
-      rewrite Min.min_l in Heqn0 by omega; subst n0.
-      destruct (le_lt_dec (length limb_widths) n). {
-        rewrite (@nth_default_out_of_bounds _ _ base) by (distr_length; auto).
-        rewrite skipn_all by (rewrite base_from_limb_widths_length; omega).
-        do 2 rewrite decode_base_nil.
-        ring_simplify; auto.
-      } {
-        rewrite (skipn_nth_default n base 0) by (distr_length; omega).
-        do 2 rewrite decode'_cons.
-        ring_simplify; ring.
-      } }
-    { rewrite (nth_default_out_of_bounds _ base) by (distr_length; omega); ring_simplify.
-      etransitivity; rewrite BaseSystem.decode'_truncate; [ reflexivity | ].
-      apply f_equal.
-      autorewrite with push_firstn simpl_update_nth.
-      rewrite update_nth_out_of_bounds by (distr_length; omega * ).
-      reflexivity. }
-  Qed.
-
-  Lemma unfold_add_to_nth n x
-    : forall xs,
-      add_to_nth n x xs
-      = match n with
-        | O => match xs with
-	       | nil => nil
-	       | x'::xs' => x + x'::xs'
-	       end
-        | S n' =>  match xs with
-		   | nil => nil
-		   | x'::xs' => x'::add_to_nth n' x xs'
-		   end
-        end.
-  Proof using Type.
-    induction n; destruct xs; reflexivity.
-  Qed.
-
-  Lemma simpl_add_to_nth_0 x
-    : forall xs,
-      add_to_nth 0 x xs
-      = match xs with
-        | nil => nil
-        | x'::xs' => x + x'::xs'
-        end.
-  Proof using Type. intro; rewrite unfold_add_to_nth; reflexivity. Qed.
-
-  Lemma simpl_add_to_nth_S x n
-    : forall xs,
-      add_to_nth (S n) x xs
-      = match xs with
-        | nil => nil
-        | x'::xs' => x'::add_to_nth n x xs'
-        end.
-  Proof using Type. intro; rewrite unfold_add_to_nth; reflexivity. Qed.
-
-  Hint Rewrite @simpl_set_nth_S @simpl_set_nth_0 : simpl_add_to_nth.
-
-  Lemma add_to_nth_cons : forall x u0 us, add_to_nth 0 x (u0 :: us) = x + u0 :: us.
-  Proof using Type. reflexivity. Qed.
-
-  Hint Rewrite @add_to_nth_cons : simpl_add_to_nth.
-
-  Lemma cons_add_to_nth : forall n f y us,
-      y :: add_to_nth n f us = add_to_nth (S n) f (y :: us).
-  Proof using Type.
-    induction n; boring.
-  Qed.
-
-  Hint Rewrite <- @cons_add_to_nth : simpl_add_to_nth.
-
-  Lemma add_to_nth_nil : forall n f, add_to_nth n f nil = nil.
-  Proof using Type.
-    induction n; boring.
-  Qed.
-
-  Hint Rewrite @add_to_nth_nil : simpl_add_to_nth.
-
-  Lemma add_to_nth_set_nth n x xs
-    : add_to_nth n x xs
-      = set_nth n (x + nth_default 0 xs n) xs.
-  Proof using Type.
-    revert xs; induction n; destruct xs;
-      autorewrite with simpl_set_nth simpl_add_to_nth;
-      try rewrite IHn;
-      reflexivity.
-  Qed.
-  Lemma add_to_nth_update_nth n x xs
-    : add_to_nth n x xs
-      = update_nth n (fun y => x + y) xs.
-  Proof using Type.
-    revert xs; induction n; destruct xs;
-      autorewrite with simpl_update_nth simpl_add_to_nth;
-      try rewrite IHn;
-      reflexivity.
-  Qed.
-
-  Lemma length_add_to_nth i x xs : length (add_to_nth i x xs) = length xs.
-  Proof using Type. unfold add_to_nth; distr_length; reflexivity. Qed.
-
-  Hint Rewrite @length_add_to_nth : distr_length.
-
-  Lemma set_nth_sum : forall n x us, (n < length us \/ n >= length limb_widths)%nat ->
-    BaseSystem.decode base (set_nth n x us) =
-    (x - nth_default 0 us n) * nth_default 0 base n + BaseSystem.decode base us.
-  Proof using Type. intros; unfold set_nth; rewrite update_nth_sum by assumption; reflexivity. Qed.
-
-  Lemma add_to_nth_sum : forall n x us, (n < length us \/ n >= length limb_widths)%nat ->
-    BaseSystem.decode base (add_to_nth n x us) =
-    x * nth_default 0 base n + BaseSystem.decode base us.
-  Proof using Type. intros; rewrite add_to_nth_set_nth, set_nth_sum; try ring_simplify; auto. Qed.
-
-  Lemma add_to_nth_nth_default_full : forall n x l i d,
-    nth_default d (add_to_nth n x l) i =
-    if lt_dec i (length l) then
-      if (eq_nat_dec i n) then x + nth_default d l i
-      else nth_default d l i
-    else d.
-  Proof using Type. intros; rewrite add_to_nth_update_nth; apply update_nth_nth_default_full; assumption. Qed.
-  Hint Rewrite @add_to_nth_nth_default_full : push_nth_default.
-
-  Lemma add_to_nth_nth_default : forall n x l i, (0 <= i < length l)%nat ->
-    nth_default 0 (add_to_nth n x l) i =
-    if (eq_nat_dec i n) then x + nth_default 0 l i else nth_default 0 l i.
-  Proof using Type. intros; rewrite add_to_nth_update_nth; apply update_nth_nth_default; assumption. Qed.
-  Hint Rewrite @add_to_nth_nth_default using omega : push_nth_default.
-
-  Lemma log_cap_nonneg : forall i, 0 <= log_cap i.
-  Proof using Type*.
-    unfold nth_default; intros.
-    case_eq (nth_error limb_widths i); intros; try omega.
-    apply limb_widths_nonneg.
-    eapply nth_error_value_In; eauto.
-  Qed. Local Hint Resolve log_cap_nonneg.
-End carrying_helper.
-
-Hint Rewrite @simpl_set_nth_S @simpl_set_nth_0 : simpl_add_to_nth.
-Hint Rewrite @add_to_nth_cons : simpl_add_to_nth.
-Hint Rewrite <- @cons_add_to_nth : simpl_add_to_nth.
-Hint Rewrite @add_to_nth_nil : simpl_add_to_nth.
-Hint Rewrite @length_add_to_nth : distr_length.
-Hint Rewrite @add_to_nth_nth_default_full : push_nth_default.
-Hint Rewrite @add_to_nth_nth_default using (omega || distr_length; omega) : push_nth_default.
-
-Section carrying.
-  Context {limb_widths} (limb_widths_nonneg : forall w, In w limb_widths -> 0 <= w).
-  Local Notation base := (base_from_limb_widths limb_widths).
-  Local Notation log_cap i := (nth_default 0 limb_widths i).
-  Local Hint Resolve limb_widths_nonneg sum_firstn_limb_widths_nonneg.
-
-  Lemma length_carry_gen : forall fc fi i us, length (carry_gen limb_widths fc fi i us) = length us.
-  Proof using Type. intros; unfold carry_gen, carry_single; distr_length; reflexivity. Qed.
-
-  Hint Rewrite @length_carry_gen : distr_length.
-
-  Lemma length_carry_simple : forall i us, length (carry_simple limb_widths i us) = length us.
-  Proof using Type. intros; unfold carry_simple; distr_length; reflexivity. Qed.
-  Hint Rewrite @length_carry_simple : distr_length.
-
-  Lemma nth_default_base_succ : forall i, (S i < length limb_widths)%nat ->
-    nth_default 0 base (S i) = 2 ^ log_cap i * nth_default 0 base i.
-  Proof using Type*.
-    intros.
-    rewrite !nth_default_base, <- Z.pow_add_r by (omega || eauto using log_cap_nonneg).
-    autorewrite with simpl_sum_firstn; reflexivity.
-  Qed.
-
-  Lemma carry_gen_decode_eq : forall fc fi i' us
-                                     (i := fi i')
-                                     (Si := fi (S i)),
-    (length us = length limb_widths) ->
-    BaseSystem.decode base (carry_gen limb_widths fc fi i' us)
-    =  (fc (nth_default 0 us i / 2 ^ log_cap i) *
-        (if eq_nat_dec Si (S i)
-         then if lt_dec (S i) (length limb_widths)
-              then 2 ^ log_cap i * nth_default 0 base i
-              else 0
-         else nth_default 0 base Si)
-        - 2 ^ log_cap i * (nth_default 0 us i / 2 ^ log_cap i) * nth_default 0 base i)
-      + BaseSystem.decode base us.
-  Proof using Type*.
-    intros fc fi i' us i Si H; intros.
-    destruct (eq_nat_dec 0 (length limb_widths));
-      [ destruct limb_widths, us, i; simpl in *; try congruence;
-        break_match;
-        unfold carry_gen, carry_single, add_to_nth;
-        autorewrite with zsimplify simpl_nth_default simpl_set_nth simpl_update_nth distr_length;
-        reflexivity
-      | ].
-    (*assert (0 <= i < length limb_widths)%nat by (subst i; auto with arith).*)
-    assert (0 <= log_cap i) by auto using log_cap_nonneg.
-    assert (2 ^ log_cap i <> 0) by (apply Z.pow_nonzero; lia).
-    unfold carry_gen, carry_single.
-     change (i' mod length limb_widths)%nat with i.
-    rewrite add_to_nth_sum by (rewrite length_set_nth; omega).
-    rewrite set_nth_sum by omega.
-    unfold Z.pow2_mod.
-    rewrite Z.land_ones by auto using log_cap_nonneg.
-    rewrite Z.shiftr_div_pow2 by auto using log_cap_nonneg.
-    change (fi i') with i.
-    subst Si.
-    repeat first [ ring
-                 | match goal with H : _ = _ |- _ => rewrite !H in * end
-                 | rewrite nth_default_base_succ by omega
-                 | rewrite !(nth_default_out_of_bounds _ base) by (distr_length; omega)
-                 | rewrite !(nth_default_out_of_bounds _ us) by omega
-                 | rewrite Z.mod_eq by assumption
-                 | progress distr_length
-                 | progress autorewrite with natsimplify zsimplify in *
-                 | progress break_match ].
-  Qed.
-
-  Lemma carry_simple_decode_eq : forall i us,
-    (length us = length limb_widths) ->
-    (i < (pred (length limb_widths)))%nat ->
-    BaseSystem.decode base (carry_simple limb_widths i us) = BaseSystem.decode base us.
-  Proof using Type*.
-    unfold carry_simple; intros; rewrite carry_gen_decode_eq by assumption.
-    autorewrite with natsimplify.
-    break_match; try lia; autorewrite with zsimplify; lia.
-  Qed.
-
-
-  Lemma length_carry_simple_sequence : forall is us, length (carry_simple_sequence limb_widths is us) = length us.
-  Proof using Type.
-    unfold carry_simple_sequence.
-    induction is; [ reflexivity | simpl; intros ].
-    distr_length.
-    congruence.
-  Qed.
-  Hint Rewrite @length_carry_simple_sequence : distr_length.
-
-  Lemma length_make_chain : forall i, length (make_chain i) = i.
-  Proof using Type. induction i; simpl; congruence. Qed.
-  Hint Rewrite @length_make_chain : distr_length.
-
-  Lemma length_full_carry_chain : length (full_carry_chain limb_widths) = length limb_widths.
-  Proof using Type. unfold full_carry_chain; distr_length; reflexivity. Qed.
-  Hint Rewrite @length_full_carry_chain : distr_length.
-
-  Lemma length_carry_simple_full us : length (carry_simple_full limb_widths us) = length us.
-  Proof using Type. unfold carry_simple_full; distr_length; reflexivity. Qed.
-  Hint Rewrite @length_carry_simple_full : distr_length.
-
-  (* TODO : move? *)
-  Lemma make_chain_lt : forall x i : nat, In i (make_chain x) -> (i < x)%nat.
-  Proof using Type.
-    induction x; simpl; intuition auto with arith lia.
-  Qed.
-
-  Lemma nth_default_carry_gen_full fc fi d i n us
-    : nth_default d (carry_gen limb_widths fc fi i us) n
-      = if lt_dec n (length us)
-        then (if eq_nat_dec n (fi i)
-              then Z.pow2_mod (nth_default 0 us n) (log_cap n)
-              else nth_default 0 us n) +
-             if eq_nat_dec n (fi (S (fi i)))
-             then fc (nth_default 0 us (fi i) >> log_cap (fi i))
-             else 0
-        else d.
-  Proof using Type.
-    unfold carry_gen, carry_single.
-    intros; autorewrite with push_nth_default natsimplify distr_length.
-    edestruct (lt_dec n (length us)) as [H|H]; [ | reflexivity ].
-    rewrite !(@nth_default_in_bounds Z 0 d) by assumption.
-    repeat break_match; subst; try omega; try rewrite_hyp *; omega.
-  Qed.
-
-  Hint Rewrite @nth_default_carry_gen_full : push_nth_default.
-
-  Lemma nth_default_carry_simple_full : forall d i n us,
-      nth_default d (carry_simple limb_widths i us) n
-      = if lt_dec n (length us)
-        then if eq_nat_dec n i
-             then Z.pow2_mod (nth_default 0 us n) (log_cap n)
-             else nth_default 0 us n +
-                  if eq_nat_dec n (S i) then nth_default 0 us i >> log_cap i else 0
-        else d.
-  Proof using Type.
-    intros; unfold carry_simple; autorewrite with push_nth_default.
-    repeat break_match; try omega; try reflexivity.
-  Qed.
-
-  Hint Rewrite @nth_default_carry_simple_full : push_nth_default.
-
-  Lemma nth_default_carry_gen
-    : forall fc fi i us,
-      (0 <= i < length us)%nat
-      -> nth_default 0 (carry_gen limb_widths fc fi i us) i
-         = (if eq_nat_dec i (fi i)
-            then Z.pow2_mod (nth_default 0 us i) (log_cap i)
-            else nth_default 0 us i) +
-           if eq_nat_dec i (fi (S (fi i)))
-           then fc (nth_default 0 us (fi i) >> log_cap (fi i))
-           else 0.
-  Proof using Type.
-    intros; autorewrite with push_nth_default natsimplify; break_match; omega.
-  Qed.
-  Hint Rewrite @nth_default_carry_gen using (omega || distr_length; omega) : push_nth_default.
-
-  Lemma nth_default_carry_simple
-    : forall i us,
-      (0 <= i < length us)%nat
-      -> nth_default 0 (carry_simple limb_widths i us) i
-         = Z.pow2_mod (nth_default 0 us i) (log_cap i).
-  Proof using Type.
-    intros; autorewrite with push_nth_default natsimplify; break_match; omega.
-  Qed.
-  Hint Rewrite @nth_default_carry_simple using (omega || distr_length; omega) : push_nth_default.
-End carrying.
-
-Hint Rewrite @length_carry_gen : distr_length.
-Hint Rewrite @length_carry_simple @length_carry_simple_sequence @length_make_chain @length_full_carry_chain @length_carry_simple_full : distr_length.
-Hint Rewrite @nth_default_carry_simple_full @nth_default_carry_gen_full : push_nth_default.
-Hint Rewrite @nth_default_carry_simple @nth_default_carry_gen using (omega || distr_length; omega) : push_nth_default.
